basis/fsFFIScript.sml
@@ -28,8 +28,8 @@ val _ = Datatype` mode = ReadMode | WriteMode`;
 *)
 
 val _ = Datatype`
-  IO_fs = <| files : (inode # char list) list ;
-             inode_tbl : (mlstring # mlstring) list;
+  IO_fs = <| inode_tbl : (inode # char list) list ;
+             files : (mlstring # mlstring) list;
              infds : (num # (inode # mode # num)) list;
              numchars : num llist;
              maxFD : num
@@ -45,7 +45,7 @@ val get_file_content_def = Define`
     get_file_content fs fd =
       do
         (fnm, md, off) <- ALOOKUP fs.infds fd ;
-        c <- ALOOKUP fs.files fnm;
+        c <- ALOOKUP fs.inode_tbl fnm;
         return (c, off)
       od`
 
@@ -61,8 +61,8 @@ val openFile_def = Define`
      in
        do
           assert (fd <= fsys.maxFD) ;
-          iname <- ALOOKUP fsys.inode_tbl fnm;
-          ALOOKUP fsys.files (File iname);
+          iname <- ALOOKUP fsys.files fnm;
+          ALOOKUP fsys.inode_tbl (File iname);
           return (fd, fsys with infds := (nextFD fsys, (File iname, md, pos)) :: fsys.infds)
        od
 `;
@@ -80,10 +80,10 @@ val openFile_truncate_def = Define`
     let fd = nextFD fsys in
       do
         assert (fd <= fsys.maxFD) ;
-        iname <- ALOOKUP fsys.inode_tbl fnm;
-        ALOOKUP fsys.files (File iname);
+        iname <- ALOOKUP fsys.files fnm;
+        ALOOKUP fsys.inode_tbl (File iname);
         return (fd, (fsys with infds := (nextFD fsys, (File iname, md, 0)) :: fsys.infds)
-                          with files updated_by (ALIST_FUPDKEY (File iname) (\x."")))
+                          with inode_tbl updated_by (ALIST_FUPDKEY (File iname) (\x."")))
       od `;
 
 (* checks if a descriptor index is in infds *)
@@ -102,7 +102,7 @@ val read_def = Define`
     do
       (fnm, md, off) <- ALOOKUP fs.infds fd ;
       assert (md = ReadMode) ;
-      content <- ALOOKUP fs.files fnm ;
+      content <- ALOOKUP fs.inode_tbl fnm ;
       strm <- LHD fs.numchars;
       let k = MIN n (MIN (LENGTH content - off) (SUC strm)) in
       return (TAKE k (DROP off content), bumpFD fd fs k)
@@ -113,7 +113,7 @@ val read_def = Define`
 val fsupdate_def = Define`
   fsupdate fs fd k pos content =
     case ALOOKUP fs.infds fd of NONE => fs | SOME (fnm,_) =>
-    (fs with <| files := ALIST_FUPDKEY fnm (K content) fs.files;
+    (fs with <| inode_tbl := ALIST_FUPDKEY fnm (K content) fs.inode_tbl;
                 numchars := THE (LDROP k fs.numchars);
                 infds := (ALIST_FUPDKEY fd (I ## I ## (K pos))) fs.infds|>)`;
 
@@ -127,7 +127,7 @@ val write_def = Define`
     do
       (fnm, md, off) <- ALOOKUP fs.infds fd ;
       assert(md = WriteMode) ;
-      content <- ALOOKUP fs.files fnm ;
+      content <- ALOOKUP fs.inode_tbl fnm ;
       assert(n <= LENGTH chars);
       assert(fs.numchars <> [||]);
       strm <- LHD fs.numchars;
@@ -186,7 +186,7 @@ val ffi_open_in_def = Define`
     od`;
 
 (* open append:
-      contents <- ALOOKUP fs.files (implode fname);
+      contents <- ALOOKUP fs.inode_tbl (implode fname);
       (fd, fs') <- openFile (implode fname) fs (LENGTH contents);
 *)
 
@@ -288,8 +288,8 @@ val encode_inode_def = Define`
   (encode_inode (UStream s) = Cons (Num 0) ((Str o explode) s)) /\
   encode_inode (File s) = Cons (Num 1) ((Str o explode) s)`;
 
-val encode_files_def = Define`
-  encode_files fs = encode_list (encode_pair encode_inode Str) fs`;
+val encode_inode_tbl_def = Define`
+  encode_inode_tbl tbl = encode_list (encode_pair encode_inode Str) tbl`;
 
 val encode_mode_def = Define`
   (encode_mode ReadMode = Num 0) ∧
@@ -299,27 +299,27 @@ val encode_fds_def = Define`
   encode_fds fds =
      encode_list (encode_pair Num (encode_pair encode_inode (encode_pair encode_mode Num))) fds`;
 
-val encode_inode_tbl_def = Define`
-  encode_inode_tbl fs = encode_list (encode_pair (Str o explode) (Str o explode)) fs`;
+val encode_files_def = Define`
+  encode_files fs = encode_list (encode_pair (Str o explode) (Str o explode)) fs`;
 
 val encode_def = zDefine`
   encode fs = Cons
                (Cons
                  (cfFFIType$Cons
                   (cfFFIType$Cons
-                    (encode_files fs.files)
+                    (encode_inode_tbl fs.inode_tbl)
                     (encode_fds fs.infds))
                   (Stream fs.numchars))
-                 (encode_inode_tbl fs.inode_tbl))
+                 (encode_files fs.files))
                (Num fs.maxFD)`
 
 Theorem encode_inode_11[simp]
   `!x y. encode_inode x = encode_inode y <=> x = y`
   (Cases \\ Cases_on `y` \\ fs [encode_inode_def,explode_11]);
 
-Theorem encode_files_11[simp]
-  `!xs ys. encode_files xs = encode_files ys <=> xs = ys`
-  (rw [] \\ eq_tac \\ rw [encode_files_def]
+Theorem encode_inode_tbl_11[simp]
+  `!xs ys. encode_inode_tbl xs = encode_inode_tbl ys <=> xs = ys`
+  (rw [] \\ eq_tac \\ rw [encode_inode_tbl_def]
   \\ drule encode_list_11
   \\ fs [encode_pair_def,FORALL_PROD,encode_inode_def]);
 
@@ -333,9 +333,9 @@ Theorem encode_fds_11[simp]
   \\ drule encode_list_11
   \\ fs [encode_pair_def,FORALL_PROD,encode_inode_def]);
 
-Theorem encode_inode_tbl_11[simp]
-  `!xs ys. encode_inode_tbl xs = encode_inode_tbl ys <=> xs = ys`
- (rw [] \\ eq_tac \\ rw [encode_inode_tbl_def]
+Theorem encode_files_11[simp]
+  `!xs ys. encode_files xs = encode_files ys <=> xs = ys`
+ (rw [] \\ eq_tac \\ rw [encode_files_def]
   \\ drule encode_list_11
   \\ fs [encode_pair_def,FORALL_PROD]);
 
