tutorial/splitwordsScript.sml
@@ -32,7 +32,7 @@ Theorem splitwords_concat_space
 
 Theorem splitwords_all_lines
   `FLAT (MAP splitwords (all_lines fs fname)) =
-   splitwords (implode (THE (ALOOKUP fs.files
+   splitwords (implode (THE (ALOOKUP fs.inode_tbl
                          (File (THE(ALOOKUP fs.file_inode fname))))))`
   `isSpace #"\n"` by EVAL_TAC \\
   rw[all_lines_def,lines_of_def,MAP_MAP_o,o_DEF,
